src/lowparse/LowParse.Low.BoundedInt.fsti
@@ -40,10 +40,24 @@ let validate_bounded_integer
 
 inline_for_extraction
 noextract
+let validate_bounded_integer_le
+  (i: integer_size) // must be a constant
+: Tot (validator (parse_bounded_integer_le i))
+= validate_total_constant_size (parse_bounded_integer_le i) (U32.uint_to_t i) ()
+
+inline_for_extraction
+noextract
 let jump_bounded_integer
   (i: integer_size) // must be a constant
 : Tot (jumper (parse_bounded_integer i))
 = jump_constant_size (parse_bounded_integer i) (U32.uint_to_t i) ()
+
+inline_for_extraction
+noextract
+let jump_bounded_integer_le
+  (i: integer_size) // must be a constant
+: Tot (jumper (parse_bounded_integer_le i))
+= jump_constant_size (parse_bounded_integer_le i) (U32.uint_to_t i) ()
 
 inline_for_extraction
 val serialize32_bounded_integer_1 : unit -> Tot (serializer32 (serialize_bounded_integer 1))
@@ -274,7 +288,23 @@ inline_for_extraction
 val read_bounded_integer_le_2 : leaf_reader (parse_bounded_integer_le 2)
 
 inline_for_extraction
+val read_bounded_integer_le_3 : leaf_reader (parse_bounded_integer_le 3)
+
+inline_for_extraction
 val read_bounded_integer_le_4 : leaf_reader (parse_bounded_integer_le 4)
+
+inline_for_extraction
+noextract
+let read_bounded_integer_le
+  (i: integer_size)
+: Tot (leaf_reader (parse_bounded_integer_le i))
+= [@inline_let]
+  let _ = integer_size_values i in
+  match i with
+  | 1 -> read_bounded_integer_le_1
+  | 2 -> read_bounded_integer_le_2
+  | 3 -> read_bounded_integer_le_3
+  | 4 -> read_bounded_integer_le_4
 
 inline_for_extraction
 val read_u16_le : leaf_reader parse_u16_le
@@ -295,6 +325,12 @@ inline_for_extraction
 val write_bounded_integer_le_2 : leaf_writer_strong (serialize_bounded_integer_le 2)
 
 inline_for_extraction
+val serialize32_bounded_integer_le_3 : serializer32 (serialize_bounded_integer_le 3)
+
+inline_for_extraction
+val write_bounded_integer_le_3 : leaf_writer_strong (serialize_bounded_integer_le 3)
+
+inline_for_extraction
 val serialize32_bounded_integer_le_4 : serializer32 (serialize_bounded_integer_le 4)
 
 inline_for_extraction
@@ -305,3 +341,74 @@ val write_u16_le : leaf_writer_strong serialize_u16_le
 
 inline_for_extraction
 val write_u32_le : leaf_writer_strong serialize_u32_le
+
+
+val validate_bounded_int32_le_1
+  (min32: U32.t)
+  (max32: U32.t { 0 < U32.v max32 /\ U32.v min32 <= U32.v max32 /\ U32.v max32 < 256 })
+: Tot (validator (parse_bounded_int32_le (U32.v min32) (U32.v max32)))
+
+val validate_bounded_int32_le_2
+  (min32: U32.t)
+  (max32: U32.t { 256 <= U32.v max32 /\ U32.v min32 <= U32.v max32 /\ U32.v max32 < 65536 })
+: Tot (validator (parse_bounded_int32_le (U32.v min32) (U32.v max32)))
+
+val validate_bounded_int32_le_3
+  (min32: U32.t)
+  (max32: U32.t { 65536 <= U32.v max32 /\ U32.v min32 <= U32.v max32 /\ U32.v max32 < 16777216 })
+: Tot (validator (parse_bounded_int32_le (U32.v min32) (U32.v max32)))
+
+val validate_bounded_int32_le_4
+  (min32: U32.t)
+  (max32: U32.t { 16777216 <= U32.v max32 /\ U32.v min32 <= U32.v max32 /\ U32.v max32 < 4294967296 })
+: Tot (validator (parse_bounded_int32_le (U32.v min32) (U32.v max32)))
+
+inline_for_extraction
+let validate_bounded_int32_le
+  (min32: U32.t)
+  (max32: U32.t { 0 < U32.v max32 /\ U32.v min32 <= U32.v max32 /\ U32.v max32 < 4294967296 })
+: Tot (validator (parse_bounded_int32_le (U32.v min32) (U32.v max32)))
+= fun #rrel #rel sl pos -> (
+  if max32 `U32.lt` 256ul
+  then validate_bounded_int32_le_1 min32 max32 sl pos
+  else if max32 `U32.lt` 65536ul
+  then validate_bounded_int32_le_2 min32 max32 sl pos
+  else if max32 `U32.lt` 16777216ul
+  then validate_bounded_int32_le_3 min32 max32 sl pos
+  else validate_bounded_int32_le_4 min32 max32 sl pos
+  )
+
+val jump_bounded_int32_le_1
+  (min32: U32.t)
+  (max32: U32.t { 0 < U32.v max32 /\ U32.v min32 <= U32.v max32 /\ U32.v max32 < 256 })
+: Tot (jumper (parse_bounded_int32_le (U32.v min32) (U32.v max32)))
+
+val jump_bounded_int32_le_2
+  (min32: U32.t)
+  (max32: U32.t { 256 <= U32.v max32 /\ U32.v min32 <= U32.v max32 /\ U32.v max32 < 65536 })
+: Tot (jumper (parse_bounded_int32_le (U32.v min32) (U32.v max32)))
+
+val jump_bounded_int32_le_3
+  (min32: U32.t)
+  (max32: U32.t { 65536 <= U32.v max32 /\ U32.v min32 <= U32.v max32 /\ U32.v max32 < 16777216 })
+: Tot (jumper (parse_bounded_int32_le (U32.v min32) (U32.v max32)))
+
+val jump_bounded_int32_le_4
+  (min32: U32.t)
+  (max32: U32.t { 16777216 <= U32.v max32 /\ U32.v min32 <= U32.v max32 /\ U32.v max32 < 4294967296 })
+: Tot (jumper (parse_bounded_int32_le (U32.v min32) (U32.v max32)))
+
+inline_for_extraction
+let jump_bounded_int32_le
+  (min32: U32.t)
+  (max32: U32.t { 0 < U32.v max32 /\ U32.v min32 <= U32.v max32 /\ U32.v max32 < 4294967296 })
+: Tot (jumper (parse_bounded_int32_le (U32.v min32) (U32.v max32)))
+= fun #rrel #rel sl pos -> (
+  if max32 `U32.lt` 256ul
+  then jump_bounded_int32_le_1 min32 max32 sl pos
+  else if max32 `U32.lt` 65536ul
+  then jump_bounded_int32_le_2 min32 max32 sl pos
+  else if max32 `U32.lt` 16777216ul
+  then jump_bounded_int32_le_3 min32 max32 sl pos
+  else jump_bounded_int32_le_4 min32 max32 sl pos
+  )
